Change the definition of safeN to accept a new parameter,   Hrel : M -> M -> prop, that holds pre/post external function calls.
In the semax, Hrel is (fun m m' => level m' < level m).
In dry semantics, Hrel = (fun m m' => True).

sepcomp/step_lemmas.v
@@ -6,13 +6,14 @@ Require Import core_semantics.
 Require Import core_semantics_lemmas.
 
 Section safety.
-  Context {G C M D Z:Type}.
+  Context {G C M Z:Type}.
+  Context {Hrel: M -> M -> Prop}.
   Context (Hcore:CoreSemantics G C M).
   Variable (Hspec:external_specification M external_function Z).
 
   Variable ge : G.
 
-  Fixpoint safeN (n:nat) (z:Z) (c:C) (m:M) : Prop :=
+  Fixpoint safeN' (n:nat) (z:Z) (c:C) (m:M) : Prop :=
     match n with
     | O => True
     | S n' => 
@@ -20,15 +21,16 @@ Section safety.
        | None, None =>
            exists c', exists m',
              corestep Hcore ge c m c' m' /\
-             safeN n' z c' m'
+             safeN' n' z c' m'
        | Some (e,sig,args), None =>
            exists x:ext_spec_type Hspec e,
              ext_spec_pre Hspec e x (sig_args sig) args z m /\
              (forall ret m' z',
+               Hrel m m' -> 
                ext_spec_post Hspec e x (sig_res sig) ret z' m' ->
                exists c',
                  after_external Hcore ret c = Some c' /\
-                 safeN n' z' c' m')
+                 safeN' n' z' c' m')
        | None, Some i => ext_spec_exit Hspec (Some i) z m
        | Some _, Some _ => False
        end
@@ -43,7 +45,7 @@ Section safety.
   Lemma safe_corestep_forward:
      corestep_fun -> 
     forall c m c' m' n z,
-    corestep Hcore ge c m c' m' -> safeN (S n) z c m -> safeN n z c' m'.
+    corestep Hcore ge c m c' m' -> safeN' (S n) z c m -> safeN' n z c' m'.
   Proof.
     simpl; intros.
     erewrite corestep_not_at_external in H1; eauto.
@@ -56,7 +58,7 @@ Section safety.
 
   Lemma safe_corestep_backward:
     forall c m c' m' n z,
-    corestep Hcore ge c m c' m' -> safeN n z c' m' -> safeN (S n) z c m.
+    corestep Hcore ge c m c' m' -> safeN' n z c' m' -> safeN' (S n) z c m.
   Proof.
     simpl; intros.
     erewrite corestep_not_at_external; eauto.
@@ -65,7 +67,7 @@ Section safety.
 
   Lemma safe_downward1 :
     forall n c m z,
-      safeN (S n) z c m -> safeN n z c m.
+      safeN' (S n) z c m -> safeN' n z c m.
   Proof.
     induction n; simpl; intros; auto.
     destruct (at_external Hcore c);
@@ -75,7 +77,7 @@ Section safety.
     destruct H as [x ?].
     exists x. 
     destruct H. split; auto.
-    intros. specialize (H0 ret m' z' H1).
+    intros. specialize (H0 ret m' z' H1 H2).
     destruct H0 as [c' [? ?]].
     exists c'; split; auto.
     auto.
@@ -86,7 +88,7 @@ Section safety.
   Lemma safe_downward : 
     forall n n' c m z,
       le n' n ->
-      safeN n z c m -> safeN n' z c m.
+      safeN' n z c m -> safeN' n' z c m.
   Proof.
     do 6 intro. revert c m z. induction H; auto.
     intros. apply IHle. apply safe_downward1. auto.
@@ -96,8 +98,8 @@ Section safety.
     corestep_fun -> 
     forall z c m c' m' n n0,
       corestepN Hcore ge n0 c m c' m' -> 
-      safeN (n + S n0) z c m -> 
-      safeN n z c' m'.
+      safeN' (n + S n0) z c m -> 
+      safeN' n z c' m'.
   Proof.
     intros.
     revert c m c' m' n H0 H1.
@@ -115,8 +117,8 @@ Section safety.
     forall
       {ora st m st' m' n},
       corestep Hcore ge st m st' m' ->
-      safeN (n-1) ora st' m' ->
-      safeN n ora st m.
+      safeN' (n-1) ora st' m' ->
+      safeN' n ora st m.
   Proof.
     intros.
     destruct n.
@@ -130,8 +132,8 @@ Section safety.
   Lemma safe_corestepN_backward:
     forall z c m c' m' n n0,
       corestepN Hcore ge n0 c m c' m' -> 
-      safeN (n - n0) z c' m' -> 
-      safeN n z c m.
+      safeN' (n - n0) z c' m' -> 
+      safeN' n z c m.
   Proof.
     simpl; intros.
     revert c m c' m' n H H0.
@@ -139,7 +141,7 @@ Section safety.
     simpl in H; inv H.
     solve[assert (Heq: (n = n - 0)%nat) by omega; rewrite Heq; auto].
     simpl in H. destruct H as [c2 [m2 [STEP STEPN]]].
-    assert (H: safeN (n - 1 - n0) z c' m'). 
+    assert (H: safeN' (n - 1 - n0) z c' m'). 
     eapply safe_downward in H0; eauto. omega.
     specialize (IHn0 _ _ _ _ (n - 1)%nat STEPN H). 
     solve[eapply safe_step'_back2; eauto].
@@ -152,7 +154,7 @@ Section safety.
                       after_external Hcore ret q2 = Some q') ->
       (halted Hcore q1 = halted Hcore q2) ->
       (forall q' m', corestep Hcore ge q1 m q' m' -> corestep Hcore ge q2 m q' m') ->
-      (forall n z, safeN n z q1 m -> safeN n z q2 m).
+      (forall n z, safeN' n z q1 m -> safeN' n z q2 m).
   Proof.
     intros. destruct n; simpl in *; auto.
     rewrite H in H3. rewrite H1 in H3.
@@ -162,7 +164,7 @@ Section safety.
     destruct H3 as [x ?].
     exists x. 
     destruct H3; split; auto.
-    intros. specialize (H4 ret m' z' H5).
+    intros. specialize (H4 ret m' z' H5 H6).
     destruct H4 as [c' [? ?]].
     exists c'; split; auto.
     destruct H3 as [c' [m' [? ?]]].
@@ -171,8 +173,8 @@ Section safety.
 
   Lemma wlog_safeN_gt0 : forall
     n z q m,
-    (lt 0 n -> safeN n z q m) -> 
-    safeN n z q m.
+    (lt 0 n -> safeN' n z q m) -> 
+    safeN' n z q m.
   Proof.
     intros. destruct n.
     hnf. auto.
@@ -180,3 +182,20 @@ Section safety.
   Qed.
 
 End safety.
+
+Require Import msl.ageable.
+
+Section juicy_safety.
+  Context {G C M Z:Type}.
+  Context `{Hage: ageable M}.
+  Context (Hcore:CoreSemantics G C M).
+  Variable (Hspec:external_specification M external_function Z).
+  Definition safeN := @safeN' G C M Z (fun m m' => (level m' < level m)%nat) Hcore Hspec.
+End juicy_safety.
+
+Section dry_safety.
+  Context {G C M Z:Type}.
+  Context (Hcore:CoreSemantics G C M).
+  Variable (Hspec:external_specification M external_function Z).
+  Definition dry_safeN := @safeN' G C M Z (fun m m' => True) Hcore Hspec.
+End dry_safety.
